Use Comparse's `is_well_formed` when possible

fstar/MLS.TreeSync.Symbolic.API.IsWellFormedInvariant.fst
@@ -1,4 +1,4 @@
-module MLS.TreeSync.Symbolic.API.HasPreInvariant
+module MLS.TreeSync.Symbolic.API.IsWellFormedInvariant
 
 open Comparse
 open MLS.Crypto
@@ -15,91 +15,91 @@ open MLS.TreeSync.API
 
 #set-options "--fuel 1 --ifuel 1"
 
-val finalize_create_has_pre:
+val is_well_formed_finalize_create:
   #bytes:Type0 -> {|crypto_bytes bytes|} -> #tkt:treekem_types bytes -> #asp:as_parameters bytes ->
   #group_id:mls_bytes bytes -> #ln:leaf_node_nt bytes tkt ->
   pre:bytes_compatible_pre bytes ->
   pend:pending_create group_id ln -> token:token_for_create asp pend -> Lemma
-  (requires value_has_pre pre ln)
+  (requires is_well_formed _ pre ln)
   (ensures (
     let new_state = finalize_create pend token in
-    treesync_has_pre pre new_state.tree
+    is_well_formed _ pre (new_state.tree <: treesync _ _ _ _)
   ))
-let finalize_create_has_pre #bytes #cb #tkt #asp #group_id #ln pre pend token =
+let is_well_formed_finalize_create #bytes #cb #tkt #asp #group_id #ln pre pend token =
   ()
 
-val finalize_welcome_has_pre:
+val is_well_formed_finalize_welcome:
   #bytes:Type0 -> {|crypto_bytes bytes|} -> #tkt:treekem_types bytes -> #asp:as_parameters bytes -> #l:nat ->
   #group_id:mls_bytes bytes -> #t:treesync bytes tkt l 0 ->
   pre:bytes_compatible_pre bytes ->
   pend:pending_welcome group_id t -> tokens:tokens_for_welcome asp pend -> Lemma
-  (requires treesync_has_pre pre t)
+  (requires is_well_formed _ pre t)
   (ensures (
     let new_state = finalize_welcome pend tokens in
-    treesync_has_pre pre new_state.tree
+    is_well_formed _ pre (new_state.tree <: treesync _ _ _ _)
   ))
-let finalize_welcome_has_pre #bytes #cb #tkt #asp #l #group_id #t pre pend tokens =
+let is_well_formed_finalize_welcome #bytes #cb #tkt #asp #l #group_id #t pre pend tokens =
   ()
 
-val finalize_add_has_pre:
+val is_well_formed_finalize_add:
   #bytes:Type0 -> {|crypto_bytes bytes|} -> #tkt:treekem_types bytes -> #asp:as_parameters bytes ->
   #st:treesync_state bytes tkt asp -> #ln:leaf_node_nt bytes tkt ->
   pre:bytes_compatible_pre bytes ->
   pend:pending_add st ln -> token:token_for_add pend -> Lemma
-  (requires treesync_has_pre pre st.tree /\ value_has_pre pre ln)
+  (requires is_well_formed _ pre (st.tree <: treesync _ _ _ _) /\ is_well_formed _ pre ln)
   (ensures (
     let (new_state, _) = finalize_add pend token in
-    treesync_has_pre pre new_state.tree
+    is_well_formed _ pre (new_state.tree <: treesync _ _ _ _)
   ))
-let finalize_add_has_pre #bytes #cb #tkt #asp #st #ln pre pend token =
+let is_well_formed_finalize_add #bytes #cb #tkt #asp #st #ln pre pend token =
   match find_empty_leaf st.tree with
   | Some li -> (
-    treesync_has_pre_tree_add pre st.tree li ln
+    is_well_formed_tree_add pre st.tree li ln
   )
   | None -> (
     find_empty_leaf_tree_extend st.tree;
     let extended_tree = tree_extend st.tree in
     let li = Some?.v (find_empty_leaf extended_tree) in
-    treesync_has_pre_tree_extend pre st.tree;
-    treesync_has_pre_tree_add pre extended_tree li ln
+    is_well_formed_tree_extend pre st.tree;
+    is_well_formed_tree_add pre extended_tree li ln
   )
 
-val finalize_update_has_pre:
+val is_well_formed_finalize_update:
   #bytes:Type0 -> {|crypto_bytes bytes|} -> #tkt:treekem_types bytes -> #asp:as_parameters bytes ->
   #st:treesync_state bytes tkt asp -> #ln:leaf_node_nt bytes tkt -> #li:treesync_index st ->
   pre:bytes_compatible_pre bytes ->
   pend:pending_update st ln li -> token:token_for_update pend -> Lemma
-  (requires treesync_has_pre pre st.tree /\ value_has_pre pre ln)
+  (requires is_well_formed _ pre (st.tree <: treesync _ _ _ _) /\ is_well_formed _ pre ln)
   (ensures (
     let new_state = finalize_update pend token in
-    treesync_has_pre pre new_state.tree
+    is_well_formed _ pre (new_state.tree <: treesync _ _ _ _)
   ))
-let finalize_update_has_pre #bytes #cb #tkt #asp #st #ln #li pre pend token =
-  treesync_has_pre_tree_update pre st.tree li ln
+let is_well_formed_finalize_update #bytes #cb #tkt #asp #st #ln #li pre pend token =
+  is_well_formed_tree_update pre st.tree li ln
 
-val finalize_remove_has_pre:
+val is_well_formed_finalize_remove:
   #bytes:Type0 -> {|crypto_bytes bytes|} -> #tkt:treekem_types bytes -> #asp:as_parameters bytes ->
   #st:treesync_state bytes tkt asp -> #li:treesync_index st ->
   pre:bytes_compatible_pre bytes ->
   pend:pending_remove st li -> Lemma
-  (requires treesync_has_pre pre st.tree)
+  (requires is_well_formed _ pre (st.tree <: treesync _ _ _ _))
   (ensures (
     let new_state = finalize_remove pend in
-    treesync_has_pre pre new_state.tree
+    is_well_formed _ pre (new_state.tree <: treesync _ _ _ _)
   ))
-let finalize_remove_has_pre #bytes #cb #tkt #asp #st #li pre pend =
+let is_well_formed_finalize_remove #bytes #cb #tkt #asp #st #li pre pend =
   //No need to prove for `truncate`? Looks like F* do it automatically
-  treesync_has_pre_tree_remove pre st.tree li
+  is_well_formed_tree_remove pre st.tree li
 
-val finalize_commit_has_pre:
+val is_well_formed_finalize_commit:
   #bytes:Type0 -> {|crypto_bytes bytes|} -> #tkt:treekem_types bytes -> #asp:as_parameters bytes ->
   #st:treesync_state bytes tkt asp -> #li:treesync_index st -> #p:pathsync bytes tkt st.levels 0 li ->
   pre:bytes_compatible_pre bytes{pre_is_hash_compatible pre} ->
   pend:pending_commit st p -> token:token_for_commit pend -> Lemma
-  (requires treesync_has_pre pre st.tree /\ pathsync_has_pre pre p)
+  (requires is_well_formed _ pre (st.tree <: treesync _ _ _ _) /\ is_well_formed _ pre p)
   (ensures (
     let new_state = finalize_commit pend token in
-    treesync_has_pre pre new_state.tree
+    is_well_formed _ pre (new_state.tree <: treesync _ _ _ _)
   ))
-let finalize_commit_has_pre #bytes #cb #tkt #asp #st #li #p pre pend token =
-  treesync_has_pre_apply_path pre st.tree p
+let is_well_formed_finalize_commit #bytes #cb #tkt #asp #st #li #p pre pend token =
+  is_well_formed_apply_path pre st.tree p
