fstar/MLS.TreeSync.Symbolic.API.KeyPackageManager.fst
@@ -28,7 +28,7 @@ let key_package_manager_types tkt = {
 val key_package_manager_pred: tkt:treekem_types dy_bytes -> map_predicate (key_package_manager_types tkt)
 let key_package_manager_pred tkt = {
   pred = (fun gu time (key_package:(key_package_manager_types tkt).key) value ->
-    value_has_pre (is_publishable gu time) key_package
+    is_well_formed _ (is_publishable gu time) key_package
   );
   pred_later = (fun gu time0 time1 key_package value -> ());
   pred_is_msg = (fun gu time key_package value -> ());
