fstar/MLS.TreeSync.Symbolic.Parsers.fst
@@ -25,3 +25,12 @@ let ps_pathsync #bytes tkt l i li =
 val ps_external_pathsync: #bytes:Type0 -> {|bytes_like bytes|} -> tkt:treekem_types bytes -> l:nat -> i:tree_index l -> li:leaf_index l i -> parser_serializer bytes (external_pathsync bytes tkt l i li)
 let ps_external_pathsync #bytes tkt l i li =
   ps_path (ps_leaf_node_data_nt tkt) (ps_option tkt.ps_node_content) l i li
+
+instance parseable_serializeable_treesync (bytes:Type0) {|bytes_like bytes|} (tkt:treekem_types bytes) (l:nat) (i:tree_index l): parseable_serializeable bytes (treesync bytes tkt l i) =
+  mk_parseable_serializeable (ps_treesync tkt l i)
+
+instance parseable_serializeable_pathsync (bytes:Type0) {|bytes_like bytes|} (tkt:treekem_types bytes) (l:nat) (i:tree_index l) (li:leaf_index l i): parseable_serializeable bytes (pathsync bytes tkt l i li) =
+  mk_parseable_serializeable (ps_pathsync tkt l i li)
+
+instance parseable_serializeable_external_pathsync (bytes:Type0) {|bytes_like bytes|} (tkt:treekem_types bytes) (l:nat) (i:tree_index l) (li:leaf_index l i): parseable_serializeable bytes (external_pathsync bytes tkt l i li) =
+  mk_parseable_serializeable (ps_external_pathsync tkt l i li)
